Fixing the main file.

concurrency/compiler/concurrent_compiler_simulation.v
@@ -25,9 +25,10 @@ Section ConcurrentCopmpilerSpecification.
   Context (Asm_program: Asm.program).
   Context (Asm_genv_safe: Asm_core.safe_genv (@the_ge Asm_program)).
 
+  Variable opt_init_mem_source: option Memory.Mem.mem.
+  Variable opt_init_mem_target: option Memory.Mem.mem.
   Definition ConcurrentCompilerCorrectness_specification: Type:=
-    forall U,
-      HybridMachine_simulation (ClightConcurSem(ge:=Clight_g) U) (@AsmConcurSem Asm_program Asm_genv_safe U).
+    HybridMachine_simulation (ClightConcurSem(ge:=Clight_g) opt_init_mem_source) (@AsmConcurSem Asm_program Asm_genv_safe opt_init_mem_target).
 
 
 End ConcurrentCopmpilerSpecification.
