concurrency/compiler/concurrent_compiler_simulation_proof.v
@@ -1,14 +1,20 @@
+Require Import compcert.common.Globalenvs.
+
 Require Import VST.concurrency.compiler.concurrent_compiler_simulation.
 Require Import VST.concurrency.compiler.sequential_compiler_correct.
 
 
 Module Concurrent_correctness (CC_correct: CompCert_correctness).
+
   
   Lemma ConcurrentCompilerCorrectness:
     forall (p:Clight.program) (tp:Asm.program),
       CC_correct.CompCert_compiler p = Some tp ->
       forall asm_genv_safety,
-        ConcurrentCompilerCorrectness_specification (Clight.globalenv p) tp asm_genv_safety.
+        ConcurrentCompilerCorrectness_specification
+          (Clight.globalenv p) tp asm_genv_safety
+          (Genv.init_mem (Ctypes.program_of_program p)) (Genv.init_mem tp)
+  .
   Proof.
     unfold ConcurrentCompilerCorrectness_specification.
     intros.
